issued, covered, reserved defs moved to IMM

src/compilation/ReserveClos.v
@@ -1,12 +1,416 @@
+Require Import Lia.
+Require Import PromisingLib.
+From Promising2 Require Import TView View Time Event Cell Thread Memory Configuration Local.
+From imm Require Import Prog.
+From imm Require Import ProgToExecution.
+From imm Require Import Events.
+From imm Require Import Execution.
+From imm Require Import imm_s.
+From imm Require Import CombRelations.
+From imm Require Import ProgToExecutionProperties.
+From imm Require Import RMWinstrProps.
+From imm Require Import AuxRel2.
+From imm Require Import FairExecution.
+From imm Require Import FinExecution.
+From imm Require Import FinThreads.
+
+Require Import SimulationRel.
+Require Import PlainStepBasic.
+Require Import SimulationPlainStep.
+Require Import MaxValue.
+Require Import SimState.
+Require Import Event_imm_promise.
+Require Import PromiseOutcome.
+Require Import CertGraphInit.
+Require Import MemoryAux.
+Require Import PromiseLTS.
+Require Import ExtSimTraversal.
+Require Import ExtSimTraversalProperties.
+Require Import ExtTraversalConfig.
+Require Import ExtTraversal.
+Require Import ExtTraversalCounting.
+Require Import SimulationPlainStepAux.
+Require Import FtoCoherent.
+Require Import AuxTime.
+Require Import IndefiniteDescription.
+From imm Require Import ImmFair. 
+Require Import Coq.Program.Basics.
+Require Import FinTravConfigs.
+Require Import ChoiceFacts.
+Require Import AuxRel. 
+Require Import ImmProperties. 
+From hahn Require Import Hahn.
+
+From imm Require Import SimTraversal.
+From imm Require Import SimTraversalProperties.
+(* From imm Require Import SimTravClosure. *)
+From imm Require Import TraversalConfigAlt.
+From imm Require Import SetSize.
+From imm Require Import SimClosure.
+
+From imm Require Import TLSCoherency.
+From imm Require Import IordCoherency. 
+Require Import TlsEventSets.
+From imm Require Import AuxDef.
+From imm Require Import TraversalOrder.
+Require Import TlsAux2.
+From imm Require Import SimIordTraversal.
+Require Import EventsTraversalOrder.
+
+Set Implicit Arguments.
+
+Section ReserveClos.
+Definition reserve_clos tc := tc ∪₁ eq ta_reserve <*> (tl_issued tc).
+
+Global Add Parametric Morphism : reserve_clos with signature
+    set_subset ==> set_subset as reserve_clos_mori.
+Proof using.
+  intros x y HH. unfold reserve_clos. rewrite HH.
+  clear. basic_solver.
+Qed. 
+
+Global Add Parametric Morphism : reserve_clos with signature
+    set_equiv ==> set_equiv as reserve_clos_more.
+Proof using.
+  intros x y [HH AA]. split.
+  { now rewrite HH. }
+  now rewrite AA.
+Qed. 
+
+(* TODO: move *)
+Lemma tl_issued_union s s' :
+  tl_issued (s ∪₁ s') ≡₁ tl_issued s ∪₁ tl_issued s'.
+Proof using. unfold tl_issued. clear. basic_solver 10. Qed.
+
+Lemma reserve_clos_union s s' :
+  reserve_clos (s ∪₁ s') ≡₁ reserve_clos s ∪₁ reserve_clos s'.
+Proof using.
+  unfold reserve_clos.
+  rewrite !tl_issued_union.
+  rewrite set_pair_union_r.
+  clear. basic_solver 10.
+Qed.
+
+
+Variable G : execution.
+Variable sc : relation actid.
+Hypothesis WF : Wf G.
+Notation "'E'" := (acts_set G).
+Notation "'W'" := (fun x => is_true (is_w (lab G) x)).
+
+(* TODO: move *)
+Lemma tl_issued_EW tc (COH : tls_coherent G tc) :
+  tl_issued tc ⊆₁ E ∩₁ W.
+Proof using WF.
+  unfold tl_issued.
+  apply set_subset_inter_r. split.
+  { apply issuedE; auto. }
+  apply issuedW; auto.
+Qed.
+
+Lemma reserve_clos_tls_coherent tc
+  (COH : tls_coherent G tc) :
+  tls_coherent G (reserve_clos tc).
+Proof using WF.
+  unfold reserve_clos.
+  apply tls_coherent_ext_union; auto.
+  unfold exec_tls.
+  arewrite (tl_issued tc ≡₁ tl_issued tc ∩₁ (is_init ∪₁ set_compl is_init)).
+  { now rewrite <- set_full_split, set_inter_full_r. }
+  rewrite tl_issued_EW; auto.
+  rewrite !set_inter_union_r, set_pair_union_r.
+  unionL.
+  { transitivity (init_tls G); eauto with hahn.
+    unfold init_tls. apply set_pair_mori; eauto with hahn.
+    clear. basic_solver. }
+  unionR right -> right.
+  apply set_pair_mori; eauto with hahn.
+  clear. basic_solver.
+Qed.
+
+Lemma reserve_clos_iord_coherent tc
+  (ICOH : iord_coherent G sc tc) :
+  iord_coherent G sc (reserve_clos tc).
+Proof using.
+  unfold reserve_clos.
+  red. rewrite id_union, seq_union_r, dom_union.
+  unionL.
+  { now unionR left. }
+  transitivity (@set_empty trav_label).
+  2: clear; basic_solver.
+  rewrite iord_no_reserve.
+  unfold set_pair.
+  unfolder. ins. do 2 desf.
+Qed.
+
+(* TODO: move *)
+Lemma reserved_ta_reserve s :
+  reserved (eq ta_reserve <*> s) ≡₁ s.
+Proof using.
+  unfold reserved.
+  unfolder; split; ins; desf.
+  { destruct y; ins. desf. }
+  eexists (_, _). splits; ins; eauto.
+Qed.
+
+(* TODO: move *)
+Lemma issued_ta_reserve s :
+  issued (eq ta_reserve <*> s) ≡₁ ∅.
+Proof using.
+  unfold issued.
+  unfolder; split; ins; desf.
+  destruct y; ins. desf.
+Qed.
+
+Local
+Hint Rewrite issued_union reserved_union
+  issued_ta_reserve reserved_ta_reserve : tc_simpl.
+
+Lemma reserve_clos_reserve_coherent tc
+  (TCOH : tls_coherent G tc)
+  (NORES : reserved tc ⊆₁ ∅) :
+  reserve_coherent G (reserve_clos tc).
+Proof using.
+  unfold reserve_clos.
+  constructor; autorewrite with tc_simpl.
+  all: repeat rewrite NORES.
+  all: repeat rewrite set_union_empty_l.
+  all: repeat rewrite set_union_empty_r.
+  { rewrite reserved_union.
+    rewrite NORES.
+    rewrite issuedE; eauto.
+    rewrite reserved_ta_reserve.
+    clear. basic_solver. }
+  { rewrite issued_union, reserved_union.
+    rewrite issued_ta_reserve.
+
+
+End ReserveClos.
+
+  
+Section ReserveClosSteps.
+
+Variable prog : Prog.t.
+Hypothesis TNONULL : ~ IdentMap.In tid_init prog.
+
+Variable G : execution.
+Variable final_memory : location -> value.
+
+Hypothesis ALLRLX  : (acts_set G) \₁ is_init ⊆₁ (fun a => is_true (is_rlx (lab G) a)).
+Hypothesis FRELACQ : (acts_set G) ∩₁ (fun a => is_true (is_f (lab G) a)) ⊆₁ (fun a => is_true (is_ra (lab G) a)).
+
+Hypothesis PROG_EX : program_execution prog G.
+Hypothesis RMWREX  : forall thread linstr
+                            (IN : Some linstr = IdentMap.find thread prog),
+    rmw_is_rex_instrs linstr.
+Hypothesis WF : Wf G.
+Variable sc : relation actid.
+Hypothesis IMMCON : imm_consistent G sc.
+
+(* TODO: doesn't it follow from PROG_EX? *)
+Hypothesis FIN_THREADS : fin_threads G.
+Hypothesis GTHREADSPROG : forall t (IN : (threads_set G \₁ eq tid_init) t), IdentMap.In t prog.
+Hypothesis THREADS_EXACT : forall t, threads_set G t <-> exists e, << ET : acts_set G e >> /\
+                                                                   << TT : t = tid e >>.
+Hypothesis EVENTS_NINIT : forall e (IN : acts_set G e) (TINIT : tid e = tid_init),
+    is_init e.
+
+Hypothesis w_ex_is_xacq : W_ex G ⊆₁ W_ex G ∩₁ is_xacq (lab G).
+
+Definition ta_label2thread (a : trav_label) : thread_id :=
+  match a with
+  | (ta_propagate t, _) => t
+  | (_, e) => tid e
+  end.
+
+Lemma isim_clos_step2ext_isim_trav_step tc1 tc2 thread tl
+  (TCOH1 : tls_coherent  G tc1)
+  (ICOH1 : iord_coherent G sc tc1)
+  (STEP : isim_clos_step G sc tl tc1 tc2)
+  (TLTOTHREAD : match tl with
+                | [] => False
+                | a :: tl => thread = ta_label2thread a
+                end) :
+  (ext_isim_trav_step G sc thread)^* (reserve_clos tc1) (reserve_clos tc2).
+Proof.
+  assert (tls_coherent G (reserve_clos tc1)) as TLSCOHTC1.
+  { apply reserve_clos_tls_coherent; auto. }
+  assert (iord_coherent G sc (reserve_clos tc1)) as ICOHTC1.
+  { apply reserve_clos_iord_coherent; auto. }
+
+  (* forward eapply sim_trav_step_coherence as COH2; eauto. *)
+  red in STEP; desf; subst.
+  { do 2 red in STEP. desf.
+    apply seq_eqv_l in STEP. destruct STEP as [STEPA STEPRES].
+    ins. apply rt_step.
+    assert (reserve_clos tc2 ≡₁ reserve_clos tc1 ∪₁ eq (ta_cover, a)) as TC2ALT.
+    { rewrite STEPRES. rewrite reserve_clos_union.
+      apply set_union_more; try easy.
+      unfold reserve_clos.
+      split.
+      2: { clear. eauto with hahn. }
+      arewrite (tl_issued (eq (ta_cover, a)) ⊆₁ ∅).
+      { unfold tl_issued. basic_solver 10. }
+      unfold set_pair. clear. unfolder. ins. do 2 desf. }
+    assert ((acts_set G \₁ is_init) a) as ENINIT.
+    { admit. }
+    assert (tls_coherent G (reserve_clos tc2)) as TLSCOHN.
+    { rewrite TC2ALT. apply tls_coherent_ext; auto.
+      red. left. red. splits; auto. }
+    destruct (lab G a) eqn:HH.
+    { apply ext_read_trav_step.
+      { type_solver. }
+      { admit. }
+      constructor; auto.
+      { apply reserve_clos_iord_coherent; auto. }
+
+
+
+
+  { apply rt_step. 
+
+  { apply rt_step. destruct tc1. simpl in *.
+    eapply ext_fence_trav_step, itrav_step2ext_itrav_step_cover; eauto. }
+  { apply rt_step. destruct tc1. simpl in *.
+    eapply ext_read_trav_step, itrav_step2ext_itrav_step_cover; eauto. }
+  { destruct tc1 as [C I] eqn:TC1. simpl in *.
+    assert (issuable G sc tc1 w) as ISS'w.
+    { inversion TS; red in H; desc; simpl in *.
+      2: congruence. 
+      destruct NEXT. apply COVEQ. basic_solver. }
+    apply itrav_step2ext_itrav_step_issue in TS as [tc' [STEPres STEP']]; auto.
+    apply seq_eqv_l in STEP' as [COH' STEP'].
+
+    destruct tc' as [[C' I'] R'].
+    assert (C' = C /\ I' = I /\ (R' = I \/ R' = I ∪₁ eq w)) as [-> [-> RES']].
+    { destruct STEPres.
+      { inversion H. auto. }
+      apply seq_eqv_r in H. desc. inversion H0. auto. }
+    assert (R' ⊆₁ I ∪₁ eq w) as RES'_.
+    { destruct RES'; basic_solver. } 
+        
+    apply rt_unit. exists [C # I # R']. split.
+    { destruct RES' as [-> | ->]; [by apply rt_refl| ]. 
+      apply rt_step. apply ext_reserve_trav_step. red. splits; vauto. }
+  
+    forward eapply ext_rlx_write_promise_step 
+      with (T := [C # I # R']) (sc := sc) as WSTEP; eauto.
+    { eapply ext_itrav_step_more; try by vauto.
+      rewrite reserved_rewrite_helper; vauto. }
+    rewrite reserved_rewrite_helper in WSTEP; vauto. }
+  { apply rt_step. destruct tc1. simpl in *.
+    eapply ext_rlx_write_cover_step, itrav_step2ext_itrav_step_cover; eauto. }
+  { destruct tc1 as [C I] eqn:TC1. simpl in *.
+
+    assert (tc_coherent G sc (mkTC C (I ∪₁ eq w))) as COH1'. 
+    { simpl. eapply trav_step_coherence; [| by apply COH1]. red. eauto. }
+
+    apply itrav_step2ext_itrav_step_issue in TS1 as [tc' [STEPres STEP']]; auto.
+    apply seq_eqv_l in STEP' as [COH' STEP'].
+    destruct tc' as [[C' I'] R'].
+    assert (C' = C /\ I' = I /\ (R' = I \/ R' = I ∪₁ eq w)) as [-> [-> RES']].
+    { destruct STEPres.
+      { inversion H. auto. }
+      apply seq_eqv_r in H. desc. inversion H0. auto. }
+    assert (R' ⊆₁ I ∪₁ eq w) as RES'_.
+    { destruct RES'; basic_solver. } 
+
+    apply rt_unit. exists [C # I # R']. split.
+    { destruct RES' as [-> | ->]; [by apply rt_refl| ]. 
+      apply rt_step. apply ext_reserve_trav_step. red. splits; vauto. }
+
+    assert (issuable G sc (mkTC C I) w) as ISS'w.
+    { apply issuable_add_eq_iff; auto.
+      apply issued_in_issuable; basic_solver. }
+  
+    forward eapply ext_rel_write_step with (T := [C # I # R']) (sc := sc)
+                                           as WSTEP; eauto.
+    { rewrite reserved_rewrite_helper; vauto. }
+    { rewrite reserved_rewrite_helper; try by vauto.
+      unfold ecovered, eissued. simpl.
+      apply itrav_step2ext_itrav_step_cover; auto. }
+    rewrite reserved_rewrite_helper in WSTEP; vauto. }  
+  { destruct tc1 as [C I] eqn:TC1. simpl in *.
+    apply rt_step. apply ext_rlx_rmw_cover_step; auto. 
+    { apply itrav_step2ext_itrav_step_cover; auto. }
+    apply itrav_step2ext_itrav_step_cover; auto.
+    unfold ecovered. simpl.
+    eapply trav_step_coherence; [| by apply COH1]. red. eauto. }
+
+  destruct tc1 as [C I] eqn:TC1. simpl in *.
+  apply rt_unit. eexists. split.
+  { replace (tid r) with (tid w).
+    2: { symmetry. erewrite wf_rmwt; eauto. }
+    apply rt_step. apply ext_reserve_trav_step. red. splits; vauto.
+    eapply etc_coh_extend_reserved_rmw; eauto.
+    { eexists. eauto. }
+    { apply coverable_add_eq_iff; auto.
+      apply covered_in_coverable.
+      { eapply trav_step_coherence; [| by apply COH1]. red. eauto. }
+      basic_solver. }
+    apply tc_coh2etc_coh; auto. }
+  
+  assert (tc_coherent G sc (mkTC (C ∪₁ eq r) I)) as COH'.
+  { eapply trav_step_coherence; [| by apply COH1]. red. eauto. }
+  assert (tc_coherent G sc (mkTC (C ∪₁ eq r) (I ∪₁ eq w))) as COH''.
+  { eapply trav_step_coherence; [| by apply COH']. red. eauto. }
+  
+  forward eapply (@reserved_rewrite_helper [C ∪₁ eq r # I # I ∪₁ eq w]) as RES_ALT; auto. 
+  { eapply etc_coh_extend_reserved_rmw; eauto.
+    { exists r. basic_solver. }
+    { apply covered_in_coverable; vauto. }
+    simpl. apply tc_coh2etc_coh; auto. }
+  { basic_solver. }
+  { apply issuable_add_eq_iff; auto.
+    apply issued_in_issuable; vauto. }
+  
+  simpl. forward eapply ext_rel_rmw_step
+    with (T := [C # I # I ∪₁ eq w]) (sc := sc) as RMWSTEP; eauto.
+  { unfold ecovered, eissued; simpl. 
+    eapply eis_add_res_rmw; eauto.
+    { basic_solver. }
+    apply itrav_step2ext_itrav_step_cover; auto. }
+  { replace (reserved [C # I # I ∪₁ eq w]) with (reserved [C ∪₁ eq r# I # I ∪₁ eq w]) by vauto.
+    replace (dom_sb_S_rfrmw G [C # I # I ∪₁ eq w]) with (dom_sb_S_rfrmw G [C ∪₁ eq r# I # I ∪₁ eq w]) by vauto.      
+    rewrite RES_ALT. 
+    
+    unfold ecovered, eissued; simpl.
+    red. splits.
+    2: { apply tc_coh2etc_coh; auto. }
+    right. left.
+    rewrite RES_ALT. 
+    unfold ecovered, eissued; simpl. splits; vauto. }    
+  { rewrite RES_ALT. unfold ecovered, eissued; simpl.
+    apply itrav_step2ext_itrav_step_cover; auto. }
+  
+  rewrite RES_ALT in RMWSTEP. auto. 
+Qed.  
+
+
+(* TODO: get rid of FRELACQ *)
+Lemma sim_clos_step2ext_sim_trav_step tc1 tc2
+      (* (COH1: tc_coherent G sc tc1) *)
+      (STEP: sim_clos_step G sc tc1 tc2)
+      (w_ex_is_xacq : W_ex G ⊆₁ W_ex G ∩₁ is_xacq (lab G)):
+  (ext_sim_trav_step G sc)^* (reserve_clos tc1) (reserve_clos tc2).
+Proof using WF IMMCON FRELACQ.
+  red in STEP. desc. 
+  apply isim_trav_step2ext_isim_trav_step in STEP; auto.
+  induction STEP.
+  { apply rt_step. red. eauto. }
+  { apply rt_refl. }
+  eapply rt_trans; eauto. 
+Qed. 
+
 
 Lemma tc_coh2etc_coh tc (COH: tc_coherent G sc tc)
       (w_ex_is_xacq : W_ex G ⊆₁ W_ex G ∩₁ is_xacq (lab G)):
-  etc_coherent G sc (mkETC tc (issued tc)). 
+  etc_coherent G sc (mkETC tc (issued tc)).
 Proof using WF IMMCON.
   forward eapply tc_coherent_implies_tc_coherent_alt as COH_ALT; eauto.
   { apply IMMCON. }
   inversion COH_ALT.
-  destruct tc as [C I]. simpl in *. 
+  destruct tc as [C I]. simpl in *.
   split; auto; unfold ecovered, eissued; simpl.
   { basic_solver. }
   { etransitivity; [| by apply tc_fwbob_I]. apply dom_rel_mori.
@@ -19,7 +423,7 @@ Proof using WF IMMCON.
     rewrite w_ex_is_xacq. forward eapply dom_wex_sb_issued as IN; eauto. }
   { sin_rewrite detour_rfe_data_rfi_rmw_rppo_in_detour_rfe_ppo; auto.
     rewrite seqA. forward eapply dom_detour_rfe_ppo_issued as IN; eauto. }
-  { rewrite (dom_l (wf_detourD WF)); auto. 
+  { rewrite (dom_l (wf_detourD WF)); auto.
     rewrite detour_in_ar, imm_s_ppo.rmw_in_ar_int, ar_int_in_ar; eauto.
     etransitivity; [| by apply tc_I_ar_rf_ppo_loc_I]. apply dom_rel_mori.
     hahn_frame. rewrite <- ct_unit, <- ct_step. apply seq_mori; basic_solver 10. }
@@ -33,10 +437,10 @@ Lemma itrav_step2ext_itrav_step_cover (C I: actid -> Prop) (e: actid)
       (STEP: itrav_step G sc e (mkTC C I) (mkTC (C ∪₁ eq e) I)):
   ext_itrav_step G sc e (mkETC (mkTC C I) I) (mkETC (mkTC (C ∪₁ eq e) I) I).
 Proof.
-  forward eapply trav_step_coherence as COH2; [by red; eauto| done |]. 
+  forward eapply trav_step_coherence as COH2; [by red; eauto| done |].
   inversion STEP.
   2: { red in H. desc. simpl in *. destruct NISS. apply ISSEQ. basic_solver. }
-  red in H. desc. red. splits; unfold ecovered, eissued; simpl in *; eauto. 
+  red in H. desc. red. splits; unfold ecovered, eissued; simpl in *; eauto.
   by apply tc_coh2etc_coh.
 Qed.
 
@@ -274,143 +678,4 @@ Proof.
   destruct NISS. apply ISSEQ, RESEQ. basic_solver. 
 Qed. 
 
-Lemma isim_trav_step2ext_isim_trav_step tc1 tc2 t
-      (COH1: tc_coherent G sc tc1)
-      (STEP: isim_trav_step G sc t tc1 tc2)
-      (w_ex_is_xacq : W_ex G ⊆₁ W_ex G ∩₁ is_xacq (lab G)):
-  (ext_isim_trav_step G sc t)^* (mkETC tc1 (issued tc1)) (mkETC tc2 (issued tc2)).
-Proof.
-  forward eapply sim_trav_step_coherence as COH2; [by red; eauto| done |]. 
-
-  inversion STEP; subst.
-  { apply rt_step. destruct tc1. simpl in *.
-    eapply ext_fence_trav_step, itrav_step2ext_itrav_step_cover; eauto. }
-  { apply rt_step. destruct tc1. simpl in *.
-    eapply ext_read_trav_step, itrav_step2ext_itrav_step_cover; eauto. }
-  { destruct tc1 as [C I] eqn:TC1. simpl in *.
-    assert (issuable G sc tc1 w) as ISS'w.
-    { inversion TS; red in H; desc; simpl in *.
-      2: congruence. 
-      destruct NEXT. apply COVEQ. basic_solver. }
-    apply itrav_step2ext_itrav_step_issue in TS as [tc' [STEPres STEP']]; auto.
-    apply seq_eqv_l in STEP' as [COH' STEP'].
-
-    destruct tc' as [[C' I'] R'].
-    assert (C' = C /\ I' = I /\ (R' = I \/ R' = I ∪₁ eq w)) as [-> [-> RES']].
-    { destruct STEPres.
-      { inversion H. auto. }
-      apply seq_eqv_r in H. desc. inversion H0. auto. }
-    assert (R' ⊆₁ I ∪₁ eq w) as RES'_.
-    { destruct RES'; basic_solver. } 
-        
-    apply rt_unit. exists [C # I # R']. split.
-    { destruct RES' as [-> | ->]; [by apply rt_refl| ]. 
-      apply rt_step. apply ext_reserve_trav_step. red. splits; vauto. }
-  
-    forward eapply ext_rlx_write_promise_step 
-      with (T := [C # I # R']) (sc := sc) as WSTEP; eauto.
-    { eapply ext_itrav_step_more; try by vauto.
-      rewrite reserved_rewrite_helper; vauto. }
-    rewrite reserved_rewrite_helper in WSTEP; vauto. }
-  { apply rt_step. destruct tc1. simpl in *.
-    eapply ext_rlx_write_cover_step, itrav_step2ext_itrav_step_cover; eauto. }
-  { destruct tc1 as [C I] eqn:TC1. simpl in *.
-
-    assert (tc_coherent G sc (mkTC C (I ∪₁ eq w))) as COH1'. 
-    { simpl. eapply trav_step_coherence; [| by apply COH1]. red. eauto. }
-
-    apply itrav_step2ext_itrav_step_issue in TS1 as [tc' [STEPres STEP']]; auto.
-    apply seq_eqv_l in STEP' as [COH' STEP'].
-    destruct tc' as [[C' I'] R'].
-    assert (C' = C /\ I' = I /\ (R' = I \/ R' = I ∪₁ eq w)) as [-> [-> RES']].
-    { destruct STEPres.
-      { inversion H. auto. }
-      apply seq_eqv_r in H. desc. inversion H0. auto. }
-    assert (R' ⊆₁ I ∪₁ eq w) as RES'_.
-    { destruct RES'; basic_solver. } 
-
-    apply rt_unit. exists [C # I # R']. split.
-    { destruct RES' as [-> | ->]; [by apply rt_refl| ]. 
-      apply rt_step. apply ext_reserve_trav_step. red. splits; vauto. }
-
-    assert (issuable G sc (mkTC C I) w) as ISS'w.
-    { apply issuable_add_eq_iff; auto.
-      apply issued_in_issuable; basic_solver. }
-  
-    forward eapply ext_rel_write_step with (T := [C # I # R']) (sc := sc)
-                                           as WSTEP; eauto.
-    { rewrite reserved_rewrite_helper; vauto. }
-    { rewrite reserved_rewrite_helper; try by vauto.
-      unfold ecovered, eissued. simpl.
-      apply itrav_step2ext_itrav_step_cover; auto. }
-    rewrite reserved_rewrite_helper in WSTEP; vauto. }  
-  { destruct tc1 as [C I] eqn:TC1. simpl in *.
-    apply rt_step. apply ext_rlx_rmw_cover_step; auto. 
-    { apply itrav_step2ext_itrav_step_cover; auto. }
-    apply itrav_step2ext_itrav_step_cover; auto.
-    unfold ecovered. simpl.
-    eapply trav_step_coherence; [| by apply COH1]. red. eauto. }
-
-  destruct tc1 as [C I] eqn:TC1. simpl in *.
-  apply rt_unit. eexists. split.
-  { replace (tid r) with (tid w).
-    2: { symmetry. erewrite wf_rmwt; eauto. }
-    apply rt_step. apply ext_reserve_trav_step. red. splits; vauto.
-    eapply etc_coh_extend_reserved_rmw; eauto.
-    { eexists. eauto. }
-    { apply coverable_add_eq_iff; auto.
-      apply covered_in_coverable.
-      { eapply trav_step_coherence; [| by apply COH1]. red. eauto. }
-      basic_solver. }
-    apply tc_coh2etc_coh; auto. }
-  
-  assert (tc_coherent G sc (mkTC (C ∪₁ eq r) I)) as COH'.
-  { eapply trav_step_coherence; [| by apply COH1]. red. eauto. }
-  assert (tc_coherent G sc (mkTC (C ∪₁ eq r) (I ∪₁ eq w))) as COH''.
-  { eapply trav_step_coherence; [| by apply COH']. red. eauto. }
-  
-  forward eapply (@reserved_rewrite_helper [C ∪₁ eq r # I # I ∪₁ eq w]) as RES_ALT; auto. 
-  { eapply etc_coh_extend_reserved_rmw; eauto.
-    { exists r. basic_solver. }
-    { apply covered_in_coverable; vauto. }
-    simpl. apply tc_coh2etc_coh; auto. }
-  { basic_solver. }
-  { apply issuable_add_eq_iff; auto.
-    apply issued_in_issuable; vauto. }
-  
-  simpl. forward eapply ext_rel_rmw_step
-    with (T := [C # I # I ∪₁ eq w]) (sc := sc) as RMWSTEP; eauto.
-  { unfold ecovered, eissued; simpl. 
-    eapply eis_add_res_rmw; eauto.
-    { basic_solver. }
-    apply itrav_step2ext_itrav_step_cover; auto. }
-  { replace (reserved [C # I # I ∪₁ eq w]) with (reserved [C ∪₁ eq r# I # I ∪₁ eq w]) by vauto.
-    replace (dom_sb_S_rfrmw G [C # I # I ∪₁ eq w]) with (dom_sb_S_rfrmw G [C ∪₁ eq r# I # I ∪₁ eq w]) by vauto.      
-    rewrite RES_ALT. 
-    
-    unfold ecovered, eissued; simpl.
-    red. splits.
-    2: { apply tc_coh2etc_coh; auto. }
-    right. left.
-    rewrite RES_ALT. 
-    unfold ecovered, eissued; simpl. splits; vauto. }    
-  { rewrite RES_ALT. unfold ecovered, eissued; simpl.
-    apply itrav_step2ext_itrav_step_cover; auto. }
-  
-  rewrite RES_ALT in RMWSTEP. auto. 
-Qed.  
-
-(* TODO: get rid of FRELACQ *)
-Lemma sim_trav_step2ext_sim_trav_step (tc1 tc2: trav_config)
-      (COH1: tc_coherent G sc tc1)
-      (STEP: sim_trav_step G sc tc1 tc2)
-      (w_ex_is_xacq : W_ex G ⊆₁ W_ex G ∩₁ is_xacq (lab G)):
-  (ext_sim_trav_step G sc)^* (mkETC tc1 (issued tc1)) (mkETC tc2 (issued tc2)).
-Proof using WF IMMCON FRELACQ.
-  red in STEP. desc. 
-  apply isim_trav_step2ext_isim_trav_step in STEP; auto.
-  induction STEP.
-  { apply rt_step. red. eauto. }
-  { apply rt_refl. }
-  eapply rt_trans; eauto. 
-Qed. 
+End ReserveClosSteps.
