src/cert_graph/TLSCoherencyAltOld.v
@@ -11,6 +11,7 @@ From imm Require Import AuxRel2.
 Require Import ExtTraversalConfig.
 From imm Require Import TraversalOrder.
 From imm Require Import TLSCoherency.
+From imm Require Import SimClosure.
 Require Import TlsEventSets.
 From imm Require Import imm_s_rfppo.
 From imm Require Import IordCoherency.
