src/ext_traversal/ExtSimTraversalProperties.v
@@ -6,6 +6,7 @@ Require Import ExtSimTraversal.
 From imm Require Import TLSCoherency.
 From imm Require Import IordCoherency.
 From imm Require Import TraversalOrder. 
+From imm Require Import SimClosure. 
 Require Import TlsEventSets.
 
 Set Implicit Arguments.
