src/reserve_steps/IssueReservedRelNextPlainStep.v
@@ -12,6 +12,7 @@ From imm Require Import CombRelations.
 From imm Require Import CombRelationsMore.
 From imm Require Import ProgToExecution.
 From imm Require Import AuxDef.
+From imm Require Import SimClosure.
 
 From imm Require Import TraversalOrder.
 From imm Require Import TLSCoherency.
