src/simulation/ViewRel.v
@@ -19,6 +19,7 @@ Require Import Event_imm_promise.
 From imm Require Import TraversalOrder.
 From imm Require Import TLSCoherency.
 From imm Require Import IordCoherency.
+From imm Require Import SimClosure.
 Require Import TlsEventSets.
 Require Import Next.
 Require Import EventsTraversalOrder.
