src/simulation_steps/ReadPlainStep.v
@@ -13,6 +13,7 @@ From imm Require Import ProgToExecution.
 From imm Require Import CombRelations CombRelationsMore.
 From imm Require Import Prog.
 From imm Require Import ProgToExecution.
+From imm Require Import SimClosure.
 
 Require Import AuxRel.
 From imm Require Import AuxRel2.
