src/tls_props/Next.v
@@ -9,6 +9,7 @@ From imm Require Import FinExecution.
 From imm Require Import TraversalOrder.
 From imm Require Import TLSCoherency.
 From imm Require Import IordCoherency.
+From imm Require Import SimClosure.
 Require Import TlsEventSets.
 Require Import EventsTraversalOrder.
 
